PumpingCfg/Utils.lean
@@ -3,7 +3,7 @@ import Mathlib.Computability.ContextFreeGrammar
 def nTimes {α : Type _} (l : List α) (n : Nat) : List α :=
   (List.replicate n l).flatten
 
-infixl:100 " ^^ " => nTimes
+infixl:100 "^^" => nTimes
 
 namespace ContextFreeGrammar
 
